Minor edit - Added comments on prop3

new/Ewflag_rid_map.fst
@@ -74,254 +74,68 @@ let concrete_merge (lca s1 s2:concrete_st) : concrete_st =
   let u = M.const_on keys (0, false) in
   M.iter_upd (fun k v -> merge_cf (sel lca k) (sel s1 k) (sel s2 k)) u
 
-let merge_pre l a b =
-  (forall id. M.contains (concrete_merge l a b) id ==>
-         fst (sel a id) >= fst (sel l id) /\
-         fst (sel b id) >= fst (sel l id))
+////////////////////////////////////////////////////////////////
+//// Linearization properties - intermediate merge //////
 
-let merge_pre' l a b =
-  (forall id. M.contains (concrete_merge l a b) id ==>
-         fst (sel a id) >= fst (sel l id) /\
-         fst (sel b id) >= fst (sel l id)) /\ // for prop5 and rec_merge
-  (forall id. (sel a id = sel b id /\ fst (sel l id) = fst (sel a id) /\ snd (sel a id) = true) ==> snd (sel l id) = true) //for rec_merge
-  
-let prop1 (l:concrete_st) (o1 o2 o3:op_t) // cond1
+let prop1 (l:concrete_st) (o1 o2 o3:op_t) 
   : Lemma (requires fst o1 <> fst o3 /\ fst o2 <> fst o3 /\ 
                     resolve_conflict o1 o3 = First_then_second /\
-                    resolve_conflict o2 o3 = First_then_second (*/\
-                    get_rid o1 = get_rid o2 /\ get_rid o3 <> get_rid o1*))
+                    resolve_conflict o2 o3 = First_then_second)
+                    //get_rid o1 = get_rid o2 /\ get_rid o3 <> get_rid o1*)
           (ensures eq (concrete_merge (do l o1) (do (do l o1) o2) (do (do l o3) o1)) (do (do (do l o3) o1) o2)) = ()
+          
+let prop2 (l s s':concrete_st) (o1 o2 o3:op_t)
+  : Lemma (requires fst o2 <> fst o3 /\ fst o1 <> fst o3 /\
+                    eq (concrete_merge l s (do l o3)) s' /\ 
+                    not (resolve_conflict o2 o3 = Second_then_first) /\
+                    not (resolve_conflict o1 o3 = Second_then_first) /\
+                    eq (concrete_merge s (do s o2) s') (do s' o2))
+          (ensures eq (concrete_merge (do s o1) (do (do s o1) o2) (do s' o1)) (do (do s' o1) o2)) = ()
 
-let prop2 (s s':concrete_st) (o1 o2:op_t) //cond2
-  : Lemma (requires //fst o1 <> fst o3 /\ fst o2 <> fst o3 /\ //extra
-                    (forall l o3. fst o2 <> fst o3 /\ eq (concrete_merge l s (do l o3)) s' ==>
-                           resolve_conflict o2 o3 = First_then_second) /\
-                    //resolve_conflict o1 o3 = First_then_second /\
-                    //resolve_conflict o2 o3 = First_then_second /\ //extra
-                    //eq (concrete_merge l s (do l o3)) s' /\ //extra
-                    eq (concrete_merge s (do s o2) s') (do s' o2) /\                    
-                    get_rid o1 = get_rid o2)
-          (ensures eq (concrete_merge (do s o1) (do (do s o1) o2) (do s' o1)) (do (do s' o1) o2)) = admit()
-
-let prop3 (l a b c:concrete_st) (op op':op_t) //cond3
-  : Lemma 
-    (requires eq (concrete_merge l a b) c /\ 
-              ((Enable? (snd (snd op)) /\ Enable? (snd (snd op'))) \/
+//prop3 requires either case analysis preconditions (or)
+//                      comment out the case analysis pre-cond and do case analysis 
+//                      on the proof like "if Disable? (snd (snd op)) then () else ()"
+let prop3 (l a b c:concrete_st) (op op':op_t)
+  : Lemma (requires eq (concrete_merge l a b) c /\ 
+              (*(Enable? (snd (snd op)) /\ Enable? (snd (snd op'))) \/
                (Enable? (snd (snd op)) /\ Disable? (snd (snd op'))) \/
                (Disable? (snd (snd op)) /\ Enable? (snd (snd op'))) \/
-               (Disable? (snd (snd op)) /\ Disable? (snd (snd op')))) /\
+               (Disable? (snd (snd op)) /\ Disable? (snd (snd op')))) /\*)
               (forall (o:op_t). eq (concrete_merge l a (do b o)) (do c o)))
               //fst op <> fst op' /\ get_rid op = get_rid op' /\
-    (ensures eq (concrete_merge l a (do (do b op) op')) (do (do c op) op')) = ()
+          (ensures eq (concrete_merge l a (do (do b op) op')) (do (do c op) op')) = 
+  if Disable? (snd (snd op)) then () else ()
 
-let prop4 (l s:concrete_st) (o1 o2 o3 o3':op_t) //automatic //cond5
+let prop4 (l s:concrete_st) (o1 o2 o3 o3':op_t)
   : Lemma (requires fst o1 <> fst o3 /\ fst o1 <> fst o3' /\ fst o2 <> fst o3 /\ fst o2 <> fst o3' /\
                     resolve_conflict o1 o3 = First_then_second /\
                     resolve_conflict o2 o3 = First_then_second /\
-                    //get_rid o1 = get_rid o2 /\ get_rid o3 = get_rid o3' /\
-                    //o3.o1, o3.o2
+                    resolve_conflict o1 o3' = First_then_second /\
                     eq (concrete_merge (do l o1) (do (do l o1) o2) (do (do s o3) o1)) (do (do (do s o3) o1) o2))
+                    //get_rid o1 = get_rid o2 /\ get_rid o3 = get_rid o3' /\
           (ensures eq (concrete_merge (do l o1) (do (do l o1) o2) (do (do (do s o3') o3) o1)) 
-                      (do (do (do (do s o3') o3) o1) o2)) = 
-  if Disable? (snd (snd o3')) then () else ()
+                      (do (do (do (do s o3') o3) o1) o2)) = ()
 
-#push-options "--z3rlimit 200"
-let rec_merge1 (s a si si' sn sn':concrete_st) (o1 o2 o3 o4:op_t)
-  : Lemma (requires eq (concrete_merge s sn sn')
-                       (concrete_merge (concrete_merge s si si') (concrete_merge s si sn') (concrete_merge s si' sn)) /\
-                    si == a /\ si' == do s o3 /\ sn == do si o2 /\ sn' == do si' o4 /\
-                    fst o2 <> fst o4 /\
-                    eq (concrete_merge s (do (do a o1) o2) sn') 
-                       (concrete_merge (do a o1) (do (do a o1) o2) (concrete_merge s (do a o1) sn')) /\
-                    eq (concrete_merge s (do (do a o1) o2) sn') 
-                       (concrete_merge si' sn' (concrete_merge s (do (do a o1) o2) si')) /\
-                    eq (concrete_merge s (do (do a o1) o2) si') 
-                       (concrete_merge (do a o1) (do (do a o1) o2) (concrete_merge s (do a o1) si')) /\
-                    eq (concrete_merge s (do a o1) sn') (concrete_merge si' sn' (concrete_merge s si' (do a o1))))
-          (ensures eq (concrete_merge s (do (do a o1) o2) sn')
-                      (concrete_merge (concrete_merge s (do a o1) si') 
-                                      (concrete_merge s (do a o1) sn') (concrete_merge s si' (do (do a o1) o2)))) = 
-  if resolve_conflict o2 o4 = First_then_second then () else ()
-
-let rec_merge_final (s a b c d:concrete_st) (o4:op_t)
-  : Lemma (requires eq (concrete_merge s b d) 
-                       (concrete_merge (concrete_merge s a c) (concrete_merge s a d) (concrete_merge s c b)) /\
-                    eq (concrete_merge s b (do d o4)) (concrete_merge a b (concrete_merge s a (do d o4))) /\
-                    eq (concrete_merge s b (do d o4)) (concrete_merge c (do d o4) (concrete_merge s b c)) /\
-                    eq (concrete_merge s b c) (concrete_merge a b (concrete_merge s a c)) /\
-                    eq (concrete_merge s a (do d o4)) (concrete_merge c (do d o4) (concrete_merge s c a)) /\
-                    eq (concrete_merge s b (do d o4)) 
-                       (concrete_merge d (concrete_merge s b d) (do d o4)))
-          (ensures eq (concrete_merge s b (do d o4))
-                      (concrete_merge (concrete_merge s a c) (concrete_merge s a (do d o4)) (concrete_merge s c b))) = 
-  if Disable? (snd (snd o4)) then () else admit()
-
-
-let rec_merge1 (s a si si' sn sn':concrete_st) (o1 o2 o3 o4:op_t)
-  : Lemma (requires eq (concrete_merge s sn sn')
-                       (concrete_merge (concrete_merge s si si') (concrete_merge s si sn') (concrete_merge s si' sn)) /\
-                    si == a /\ si' == do s o3 /\ sn == do si o2 /\ sn' == do si' o4 /\
-                    fst o2 <> fst o4 /\
-                    eq (concrete_merge s (do (do a o1) o2) sn') 
-                       (concrete_merge (do a o1) (do (do a o1) o2) (concrete_merge s (do a o1) sn')) /\
-                    eq (concrete_merge s (do (do a o1) o2) sn') 
-                       (concrete_merge si' sn' (concrete_merge s (do (do a o1) o2) si')) /\
-                    eq (concrete_merge s (do (do a o1) o2) si') 
-                       (concrete_merge (do a o1) (do (do a o1) o2) (concrete_merge s (do a o1) si')) /\
-                    eq (concrete_merge s (do a o1) sn') (concrete_merge si' sn' (concrete_merge s si' (do a o1))))
-          (ensures eq (concrete_merge s (do (do a o1) o2) sn')
-                      (concrete_merge (concrete_merge s (do a o1) si') 
-                                      (concrete_merge s (do a o1) sn') (concrete_merge s si' (do (do a o1) o2)))) = 
-  if resolve_conflict o2 o4 = First_then_second then () else ()
-  
-
-let rec_merge1 (s a:concrete_st) (o1 o2 o3 o4:op_t)
-  : Lemma (requires eq (concrete_merge s (do a o2) (do (do s o3) o4))
-                       (concrete_merge (concrete_merge s a (do s o3)) 
-                                       (concrete_merge s a (do (do s o3) o4)) 
-                                       (concrete_merge s (do s o3) (do a o2))) /\
-                    //get_rid o1 = get_rid o2 /\ get_rid o3 = get_rid o4 /\ get_rid o1 <> get_rid o3 /\
-                    //fst o2 <> fst o4 /\ fst o2 <> fst o3 /\
-                    //resolve_conflict o2 o4 = Second_then_first /\ resolve_conflict o2 o3 = Second_then_first /\ //done
-                    //resolve_conflict o2 o4 = First_then_second /\ //done
-                    //resolve_conflict o2 o4 = Second_then_first /\ //done
-                    eq (concrete_merge s (do (do a o1) o2) (do (do s o3) o4)) 
-                       (concrete_merge (do a o1) (do (do a o1) o2) (concrete_merge s (do a o1) (do (do s o3) o4))) /\
-                    eq (concrete_merge s (do (do a o1) o2) (do (do s o3) o4)) 
-                       (concrete_merge (do s o3) (do (do s o3) o4) (concrete_merge s (do (do a o1) o2) (do s o3))) /\
-                    eq (concrete_merge s (do (do a o1) o2) (do s o3)) 
-                       (concrete_merge (do a o1) (do (do a o1) o2) (concrete_merge s (do a o1) (do s o3))) /\
-                    eq (concrete_merge s (do a o1) (do (do s o3) o4)) 
-                       (concrete_merge (do s o3) (do (do s o3) o4) (concrete_merge s (do s o3) (do a o1))))
-          (ensures eq (concrete_merge s (do (do a o1) o2) (do (do s o3) o4))
-                      (concrete_merge (concrete_merge s (do a o1) (do s o3)) 
-                                      (concrete_merge s (do a o1) (do (do s o3) o4)) 
-                                      (concrete_merge s (do s o3) (do (do a o1) o2)))) = ()
-
+////////////////////////////////////////////////////////////////
+//// Recursive merge condition //////
 
 let merge_pre l a b =
   (forall id. M.contains (concrete_merge l a b) id ==>
          fst (sel a id) >= fst (sel l id) /\
          fst (sel b id) >= fst (sel l id))
-
-#push-options "--z3rlimit 200"
-let merge_pre' l a b =
-  (forall id. M.contains (concrete_merge l a b) id ==>
-         fst (sel a id) >= fst (sel l id) /\
-         fst (sel b id) >= fst (sel l id)) /\ // for prop5 and rec_merge
-  (forall id. (sel a id = sel b id /\ fst (sel l id) = fst (sel a id) /\ snd (sel a id) = true) ==> snd (sel l id) = true) //for rec_merge
-
-let pre_sep l a = 
-  (forall id. (M.contains l id \/ M.contains a id) ==>
-         fst (sel a id) >= fst (sel l id))
-
+         
 let rec_merge (s si si' sn sn':concrete_st)
-  : Lemma (requires //merge_pre' s sn sn' /\ merge_pre' si sn sn' /\ merge_pre' si' sn sn' /\ 
-                    //merge_pre' s sn si' /\ merge_pre' s si sn' /\
-                    //merge_pre' s si si' /\ merge_pre' s si' si /\ 
-                    //eq (concrete_merge si si sn) sn /\ eq (concrete_merge si' si' sn') sn' /\
-                    pre_sep si sn /\ //pre_sep si' sn' /\ 
-                    pre_sep si (concrete_merge s si si') /\ pre_sep si' (concrete_merge s si' si) /\
-                    //merge_pre si sn (concrete_merge s si si') /\ merge_pre si' sn' (concrete_merge s si' si) /\
-                    //merge_pre' (concrete_merge s si si') (concrete_merge s si sn') (concrete_merge s si' sn) /\
-                    //merge_pre' si sn (concrete_merge s si sn') /\ merge_pre' si' (concrete_merge s sn si') sn' /\
-
-                    //eq (concrete_merge s si si') (concrete_merge s (concrete_merge s s si) si') /\
-                    //eq (concrete_merge s si si') (concrete_merge s (concrete_merge s s si') si) /\
+  : Lemma (requires //merge_pre s sn sn' /\ merge_pre s sn si' /\ merge_pre s si sn' /\ merge_pre s si' sn /\
+                    //merge_pre s si si' /\ merge_pre s si' si /\ 
+                    merge_pre si sn (concrete_merge s si si') /\ merge_pre si' sn' (concrete_merge s si' si) /\
+                    //merge_pre (concrete_merge s si si') (concrete_merge s si sn') (concrete_merge s si' sn) /\
+                    //merge_pre si sn (concrete_merge s si sn') /\ merge_pre si' sn' (concrete_merge s sn si') /\
+                    
                     eq (concrete_merge s sn sn') (concrete_merge si sn (concrete_merge s si sn')) /\
                     eq (concrete_merge s sn sn') (concrete_merge si' sn' (concrete_merge s sn si')) /\
-                    eq (concrete_merge s sn si') (concrete_merge si sn (concrete_merge s si si')) /\
-                    eq (concrete_merge s si sn') (concrete_merge si' sn' (concrete_merge s si' si)))
-         
+                    //eq (concrete_merge s sn si') (concrete_merge si sn (concrete_merge s si si')) /\
+                    eq (concrete_merge s si sn') (concrete_merge si' sn' (concrete_merge s si' si)))         
           (ensures (eq (concrete_merge s sn sn')
                        (concrete_merge (concrete_merge s si si') (concrete_merge s si sn') (concrete_merge s si' sn)))) = ()
-                       
-let rec_merge1 (s si si' sn sn':concrete_st)
-  : Lemma (requires merge_pre' s sn sn' /\ merge_pre' si sn sn' /\ merge_pre' si' sn sn' /\ 
-                    merge_pre' s sn si' /\ merge_pre' s si sn' /\
-                    merge_pre' s si si' /\ merge_pre' s si' si /\ 
-                    merge_pre' si sn (concrete_merge s si si') /\ merge_pre' si' sn' (concrete_merge s si' si) /\
-                    merge_pre' (concrete_merge s si si') (concrete_merge s si sn') (concrete_merge s si' sn) /\
-                    eq (concrete_merge s sn sn') (concrete_merge si sn sn') /\
-                    eq (concrete_merge s sn sn') (concrete_merge si' sn sn') /\
-                    eq (concrete_merge s sn si') (concrete_merge si sn (concrete_merge s si si')) /\
-                    eq (concrete_merge s si sn') (concrete_merge si' sn' (concrete_merge s si' si)))
-          (ensures (eq (concrete_merge s sn sn')
-                       (concrete_merge (concrete_merge s si si') (concrete_merge s si sn') (concrete_merge s si' sn)))) = ()
-
-
-(*#push-options "--z3rlimit 100"
-let prop1 (l:concrete_st) (o1 o2 o3:op_t) // cond1
-  : Lemma (requires fst o1 <> fst o3 /\ fst o2 <> fst o3 /\ 
-                    not (resolve_conflict o3 o1 = First_then_second) /\
-                    not (resolve_conflict o3 o2 = First_then_second) /\
-                    get_rid o1 = get_rid o2 (*/\ get_rid o3 <> get_rid o1*))
-                    //resolve_conflict o1 o3 = First_then_second) //o3.o1
-                    //not (resolve_conflict o2 o3 = Second_then_first) //not(o2.o3)
-          (ensures eq (concrete_merge (do l o1) (do (do l o1) o2) (do (do l o3) o1)) (do (do (do l o3) o1) o2)) = ()
-
-let prop2 (l s s':concrete_st) (o1 o2 o3:op_t) //cond2
-  : Lemma (requires eq (concrete_merge s (do s o2) s') (do s' o2) /\
-                    fst o1 <> fst o3 /\ fst o2 <> fst o3 /\
-                    //not (resolve_conflict o3 o1 = First_then_second) /\
-                    not (resolve_conflict o3 o2 = First_then_second) /\
-                    eq (concrete_merge l s (do l o3)) s' //extra
-                    (*get_rid o1 = get_rid o2 /\ get_rid o1 <> get_rid o3*))
-          (ensures eq (concrete_merge (do s o1) (do (do s o1) o2) (do s' o1)) (do (do s' o1) o2)) = ()
-
-let prop3 (s s':concrete_st) (o2 o2':op_t)
-  : Lemma (requires eq (concrete_merge s s s') s' /\
-                    ((Enable? (snd (snd o2)) /\ Enable? (snd (snd o2'))) \/
-                     (Enable? (snd (snd o2)) /\ Disable? (snd (snd o2'))) \/
-                     (Disable? (snd (snd o2)) /\ Enable? (snd (snd o2'))) \/
-                     (Disable? (snd (snd o2)) /\ Disable? (snd (snd o2')))) /\
-                    (forall o. eq (concrete_merge s (do s o) s') (do s' o)) /\
-                    fst o2 <> fst o2' /\ get_rid o2 = get_rid o2')
-          (ensures eq (concrete_merge s (do (do s o2') o2) s') (do (do s' o2') o2)) = ()
-
-let lem_merge3 (l a b c:concrete_st) (op op':op_t) //cond3
-  : Lemma 
-    (requires eq (concrete_merge l a b) c /\ 
-              ((Enable? (snd (snd op)) /\ Enable? (snd (snd op'))) \/
-               (Enable? (snd (snd op)) /\ Disable? (snd (snd op'))) \/
-               (Disable? (snd (snd op)) /\ Enable? (snd (snd op'))) \/
-               (Disable? (snd (snd op)) /\ Disable? (snd (snd op')))) /\
-              //fst op <> fst op' /\ get_rid op = get_rid op' /\
-              (forall (o:op_t). eq (concrete_merge l a (do b o)) (do c o)))
-    (ensures eq (concrete_merge l a (do (do b op) op')) (do (do c op) op')) = ()
-
-let prop4 (l s:concrete_st) (o1 o2 o3 o3':op_t) //automatic //cond5
-  : Lemma (requires fst o1 <> fst o3 /\ fst o1 <> fst o3' /\ fst o2 <> fst o3 /\ fst o2 <> fst o3' /\
-                    //not (resolve_conflict o3 o1 = First_then_second) /\
-                    //not (resolve_conflict o3' o1 = First_then_second) /\
-                    //not (resolve_conflict o3 o2 = First_then_second) /\
-                    not (resolve_conflict o3' o2 = First_then_second) /\
-                    eq (concrete_merge l (do (do l o1) o2) s) (do (do s o1) o2) /\
-                    (*get_rid o1 = get_rid o2 /\*) get_rid o3 = get_rid o3' /\
-                    //o3.o1, o3'.o1, o3.o2, o3'.o2
-                    eq (concrete_merge (do l o1) (do (do l o1) o2) (do (do s o3) o1)) (do (do (do s o3) o1) o2))
-          (ensures eq (concrete_merge (do l o1) (do (do l o1) o2) (do (do (do s o3') o3) o1)) 
-                      (do (do (do (do s o3') o3) o1) o2)) = ()
-
-let lem_merge4 (s s':concrete_st) (op op':op_t) //cond4
-  : Lemma (requires get_rid op = get_rid op' /\
-                    ((Enable? (snd (snd op)) /\ Enable? (snd (snd op'))) \/
-                    (Enable? (snd (snd op)) /\ Disable? (snd (snd op'))) \/
-                    (Disable? (snd (snd op)) /\ Enable? (snd (snd op'))) \/
-                    (Disable? (snd (snd op)) /\ Disable? (snd (snd op')))) /\
-                    eq (concrete_merge (do s op) (do s' op) (do s op)) (do s' op))
-          (ensures eq (concrete_merge (do s op) (do (do s' op') op) (do s op)) (do (do s' op') op)) = ()
-
-let idempotence (s:concrete_st) //automatic
-  : Lemma (eq (concrete_merge s s s) s) = ()
-
-let prop5' (l s s':concrete_st) (o o3:op_t)
-  : Lemma (requires eq (concrete_merge s s s') s' /\
-                    eq (concrete_merge l s (do l o3)) s' /\ //extra
-                    ((Enable? (snd (snd o)) /\ Enable? (snd (snd o3))) \/
-                    (Enable? (snd (snd o)) /\ Disable? (snd (snd o3))) \/
-                    (Disable? (snd (snd o)) /\ Enable? (snd (snd o3))) \/
-                    (Disable? (snd (snd o)) /\ Disable? (snd (snd o3)))) /\
-                    get_rid o <> get_rid o3)
-          (ensures eq (concrete_merge s s (do s' o)) (do s' o)) = ()
-#pop-options*)
+          
+////////////////////////////////////////////////////////////////
