new/ORSet_rid_map.fst
@@ -70,167 +70,68 @@ let concrete_merge (lca s1 s2:concrete_st) : concrete_st =
   let u = M.const_on eles init_st in
   M.iter_upd (fun k v -> E.concrete_merge (sel lca k) (sel s1 k) (sel s2 k)) u
 
-let prop1 (l:concrete_st) (o1 o2 o3:op_t) // cond1
+////////////////////////////////////////////////////////////////
+//// Linearization properties - intermediate merge //////
+
+let prop1 (l:concrete_st) (o1 o2 o3:op_t)
   : Lemma (requires fst o1 <> fst o3 /\ fst o2 <> fst o3 /\ 
                     resolve_conflict o1 o3 = First_then_second /\
-                    resolve_conflict o2 o3 = First_then_second (*/\
-                    get_rid o1 = get_rid o2 /\ get_rid o3 <> get_rid o1*))
+                    resolve_conflict o2 o3 = First_then_second)
+                    //get_rid o1 = get_rid o2 /\ get_rid o3 <> get_rid o1*))
           (ensures eq (concrete_merge (do l o1) (do (do l o1) o2) (do (do l o3) o1)) (do (do (do l o3) o1) o2)) = ()
 
 #push-options "--z3rlimit 50"
-let prop2 (s s':concrete_st) (o1 o2 o3:op_t) //cond2
-  : Lemma (requires fst o1 <> fst o3 /\ fst o2 <> fst o3 /\
-                    resolve_conflict o1 o3 = First_then_second /\
-                    resolve_conflict o2 o3 = First_then_second /\
-                    eq (concrete_merge s (do s o2) s') (do s' o2)
-                    (*get_rid o1 = get_rid o2 /\ get_rid o1 <> get_rid o3*))
+let prop2 (l s s':concrete_st) (o1 o2 o3:op_t)
+  : Lemma (requires fst o2 <> fst o3 /\ fst o1 <> fst o3 /\
+                    eq (concrete_merge l s (do l o3)) s' /\
+                    not (resolve_conflict o2 o3 = Second_then_first) /\ 
+                    not (resolve_conflict o1 o3 = Second_then_first) /\
+                    eq (concrete_merge s (do s o2) s') (do s' o2))
           (ensures eq (concrete_merge (do s o1) (do (do s o1) o2) (do s' o1)) (do (do s' o1) o2)) = ()
 
-let prop3 (l a b c:concrete_st) (op op':op_t) //cond3
-  : Lemma 
-    (requires eq (concrete_merge l a b) c /\ 
+//prop3 requires case analysis pre-conditions
+let prop3 (l a b c:concrete_st) (op op':op_t) 
+  : Lemma (requires eq (concrete_merge l a b) c /\ 
               ((Add? (snd (snd op)) /\ Add? (snd (snd op'))) \/
                (Add? (snd (snd op)) /\ Rem? (snd (snd op'))) \/
                (Rem? (snd (snd op)) /\ Add? (snd (snd op'))) \/
                (Rem? (snd (snd op)) /\ Rem? (snd (snd op')))) /\
               (forall (o:op_t). eq (concrete_merge l a (do b o)) (do c o)))
               //fst op <> fst op' /\ get_rid op = get_rid op' /\
-    (ensures eq (concrete_merge l a (do (do b op) op')) (do (do c op) op')) = ()
+          (ensures eq (concrete_merge l a (do (do b op) op')) (do (do c op) op')) = ()
 
-let prop4 (l s:concrete_st) (o1 o2 o3 o3':op_t) //automatic //cond5
+let prop4 (l s:concrete_st) (o1 o2 o3 o3':op_t)
   : Lemma (requires fst o1 <> fst o3 /\ fst o1 <> fst o3' /\ fst o2 <> fst o3 /\ fst o2 <> fst o3' /\
                     resolve_conflict o1 o3 = First_then_second /\
                     resolve_conflict o2 o3 = First_then_second /\
-                    not (resolve_conflict o2 o3' = Second_then_first) /\ //extra ----- check
-                    //get_rid o1 = get_rid o2 /\ get_rid o3 = get_rid o3' /\ get_rid o1 <> get_rid o3 /\
+                    resolve_conflict o1 o3' = First_then_second /\
                     eq (concrete_merge (do l o1) (do (do l o1) o2) (do (do s o3) o1)) (do (do (do s o3) o1) o2))
+                    //get_rid o1 = get_rid o2 /\ get_rid o3 = get_rid o3' /\
           (ensures eq (concrete_merge (do l o1) (do (do l o1) o2) (do (do (do s o3') o3) o1)) 
                       (do (do (do (do s o3') o3) o1) o2)) = ()
+  
+////////////////////////////////////////////////////////////////
+//// Recursive merge condition //////
 
 let merge_pre l a b =
   (forall e. M.contains (concrete_merge l a b) e ==>
         (forall id. M.contains (sel (concrete_merge l a b) e) id ==>
                fst (E.sel (sel a e) id) >= fst (E.sel (sel l e) id) /\
                fst (E.sel (sel b e) id) >= fst (E.sel (sel l e) id)))
-               
-#push-options "--z3rlimit 200"
-let merge_pre' l a b =
-  (forall e. M.contains (concrete_merge l a b) e ==>
-        (forall id. M.contains (sel (concrete_merge l a b) e) id ==>
-               fst (E.sel (sel a e) id) >= fst (E.sel (sel l e) id) /\
-               fst (E.sel (sel b e) id) >= fst (E.sel (sel l e) id))) /\
-  (forall e id. (E.sel (sel a e) id = E.sel (sel b e) id /\ fst (E.sel (sel l e) id) = fst (E.sel (sel a e) id) /\ 
-           snd (E.sel (sel a e) id) = true) ==> snd (E.sel (sel l e) id) = true)
 
+#push-options "--z3rlimit 100"
 let rec_merge (s si si' sn sn':concrete_st)
-  : Lemma (requires //merge_pre' s sn sn' /\ merge_pre' si sn sn' /\ merge_pre' si' sn sn' /\ 
-                    //merge_pre' s sn si' /\ merge_pre' s si sn' /\
-                    //merge_pre' s si si' /\ merge_pre' s si' si /\ 
+  : Lemma (requires //merge_pre s sn sn' /\ merge_pre s sn si' /\ merge_pre s si sn' /\ merge_pre s si' sn /\
+                    //merge_pre s si si' /\ merge_pre s si' si /\ 
                     merge_pre si sn (concrete_merge s si si') /\ merge_pre si' sn' (concrete_merge s si' si) /\
-                    //merge_pre' (concrete_merge s si si') (concrete_merge s si sn') (concrete_merge s si' sn) /\
-                    //merge_pre' si sn (concrete_merge s si sn') /\ merge_pre' si' (concrete_merge s sn si') sn' /\
+                    //merge_pre (concrete_merge s si si') (concrete_merge s si sn') (concrete_merge s si' sn) /\
+                    //merge_pre si sn (concrete_merge s si sn') /\ merge_pre si' sn' (concrete_merge s sn si') /\
                     
                     eq (concrete_merge s sn sn') (concrete_merge si sn (concrete_merge s si sn')) /\
-                    eq (concrete_merge s sn sn') (concrete_merge si' (concrete_merge s sn si') sn') /\
+                    eq (concrete_merge s sn sn') (concrete_merge si' sn' (concrete_merge s sn si')) /\
                     eq (concrete_merge s sn si') (concrete_merge si sn (concrete_merge s si si')) /\
-                    eq (concrete_merge s si sn') (concrete_merge si' sn' (concrete_merge s si' si)))
-         
+                    eq (concrete_merge s si sn') (concrete_merge si' sn' (concrete_merge s si' si)))         
           (ensures (eq (concrete_merge s sn sn')
                        (concrete_merge (concrete_merge s si si') (concrete_merge s si sn') (concrete_merge s si' sn)))) = ()
-                      
-let rec_merge1 (s si si' sn sn':concrete_st)
-  : Lemma (requires merge_pre' s sn sn' /\ merge_pre' si sn sn' /\ merge_pre' si' sn sn' /\ 
-                    merge_pre' s sn si' /\ merge_pre' s si sn' /\
-                    merge_pre' s si si' /\ merge_pre' s si' si /\ 
-                    merge_pre' si sn (concrete_merge s si si') /\ merge_pre' si' sn' (concrete_merge s si' si) /\
-                    merge_pre' (concrete_merge s si si') (concrete_merge s si sn') (concrete_merge s si' sn) /\
-                    eq (concrete_merge s sn sn') (concrete_merge si sn sn') /\
-                    eq (concrete_merge s sn sn') (concrete_merge si' sn sn') /\
-                    eq (concrete_merge s sn si') (concrete_merge si sn (concrete_merge s si si')) /\
-                    eq (concrete_merge s si sn') (concrete_merge si' sn' (concrete_merge s si' si)))
-          (ensures (eq (concrete_merge s sn sn')
-                       (concrete_merge (concrete_merge s si si') (concrete_merge s si sn') (concrete_merge s si' sn)))) = ()
-                       
-(*#push-options "--z3rlimit 100"
-let prop1 (l:concrete_st) (o1 o2 o3:op_t) // cond1
-  : Lemma (requires fst o1 <> fst o3 /\ fst o2 <> fst o3 /\ 
-                    not (resolve_conflict o3 o1 = First_then_second) /\
-                    not (resolve_conflict o3 o2 = First_then_second) /\
-                    get_rid o1 = get_rid o2 (*/\ get_rid o3 <> get_rid o1*))
-                    //resolve_conflict o1 o3 = First_then_second) //o3.o1
-                    //not (resolve_conflict o2 o3 = Second_then_first) //not(o2.o3)
-          (ensures eq (concrete_merge (do l o1) (do (do l o1) o2) (do (do l o3) o1)) (do (do (do l o3) o1) o2)) = ()
 
-let prop2 (l s s':concrete_st) (o1 o2 o3:op_t) //cond2
-  : Lemma (requires eq (concrete_merge s (do s o2) s') (do s' o2) /\
-                    fst o1 <> fst o3 /\ fst o2 <> fst o3 /\
-                    not (resolve_conflict o3 o1 = First_then_second) /\
-                    not (resolve_conflict o3 o2 = First_then_second) /\
-                    eq (concrete_merge l s (do l o3)) s'
-                    (*get_rid o1 = get_rid o2 /\ get_rid o1 <> get_rid o3*))
-          (ensures eq (concrete_merge (do s o1) (do (do s o1) o2) (do s' o1)) (do (do s' o1) o2)) = ()
-          
-let prop3 (s s':concrete_st) (o2 o2':op_t) 
-  : Lemma (requires eq (concrete_merge s s s') s' /\
-                    ((Add? (snd (snd o2)) /\ Add? (snd (snd o2'))) \/
-                     (Add? (snd (snd o2)) /\ Rem? (snd (snd o2'))) \/
-                     (Rem? (snd (snd o2)) /\ Add? (snd (snd o2'))) \/
-                     (Rem? (snd (snd o2)) /\ Rem? (snd (snd o2')))) /\
-                    (forall o. eq (concrete_merge s (do s o) s') (do s' o)) /\
-                    fst o2 <> fst o2' /\ get_rid o2 = get_rid o2')
-          (ensures eq (concrete_merge s (do (do s o2') o2) s') (do (do s' o2') o2)) = ()
-
-let lem_merge3 (l a b c:concrete_st) (op op':op_t) //cond3
-  : Lemma 
-    (requires eq (concrete_merge l a b) c /\ 
-              ((Add? (snd (snd op)) /\ Add? (snd (snd op'))) \/
-               (Add? (snd (snd op)) /\ Rem? (snd (snd op'))) \/
-               (Rem? (snd (snd op)) /\ Add? (snd (snd op'))) \/
-               (Rem? (snd (snd op)) /\ Rem? (snd (snd op')))) /\
-              //fst op <> fst op' /\ get_rid op = get_rid op' /\
-              (forall (o:op_t). eq (concrete_merge l a (do b o)) (do c o)))
-    (ensures eq (concrete_merge l a (do (do b op) op')) (do (do c op) op')) = ()
-
-let merge_pre l a b =
-  (forall e. M.contains (concrete_merge l a b) e ==>
-        (forall id. M.contains (sel (concrete_merge l a b) e) id ==>
-               fst (E.sel (sel a e) id) >= fst (E.sel (sel l e) id) /\
-               fst (E.sel (sel b e) id) >= fst (E.sel (sel l e) id)))
-
-let prop4 (l s:concrete_st) (o1 o2 o3 o3':op_t)  //cond5
-  : Lemma (requires fst o1 <> fst o3 /\ fst o1 <> fst o3' /\ fst o2 <> fst o3 /\ fst o2 <> fst o3' /\
-                    //merge_pre (do l o1) (do (do l o1) o2) (do (do s o3) o1) /\
-                    //merge_pre (do l o1) (do (do l o1) o2) (do (do (do s o3') o3) o1) /\
-                    //not (resolve_conflict o3 o1 = First_then_second) /\
-                     (resolve_conflict o2 o3 = First_then_second) /\
-                     //not (resolve_conflict o3' o1 = First_then_second) /\
-                    resolve_conflict o3' o2 = First_then_second /\
-                    get_rid o1 = get_rid o2 /\ get_rid o3 = get_rid o3' /\
-                    //o3.o1, o3'.o1, o3.o2, o3'.o2
-                    eq (concrete_merge (do l o1) (do (do l o1) o2) (do (do s o3) o1)) (do (do (do s o3) o1) o2))
-          (ensures eq (concrete_merge (do l o1) (do (do l o1) o2) (do (do (do s o3') o3) o1)) 
-                      (do (do (do (do s o3') o3) o1) o2)) = ()
-
-let lem_merge4 (s s':concrete_st) (op op':op_t) //cond4
-  : Lemma (requires get_rid op = get_rid op' /\
-                    merge_pre (do s op) (do s' op) (do s op) /\ //extra pre-cond
-                    ((Add? (snd (snd op)) /\ Add? (snd (snd op'))) \/ 
-                    (Add? (snd (snd op)) /\ Rem? (snd (snd op'))) \/ 
-                    (Rem? (snd (snd op)) /\ Add? (snd (snd op'))) \/ 
-                    (Rem? (snd (snd op)) /\ Rem? (snd (snd op')))) /\ 
-                    eq (concrete_merge (do s op) (do s' op) (do s op)) (do s' op))
-          (ensures eq (concrete_merge (do s op) (do (do s' op') op) (do s op)) (do (do s' op') op)) = ()
-
-let idempotence (s:concrete_st) 
-  : Lemma (eq (concrete_merge s s s) s) = ()
-
-let prop5' (l s s':concrete_st) (o o3:op_t)
-  : Lemma (requires eq (concrete_merge s s s') s' /\
-                    merge_pre s s s' /\
-                    //eq (concrete_merge l s (do l o3)) s' /\
-                    ((Add? (snd (snd o)) /\ Add? (snd (snd o3))) \/
-                    (Add? (snd (snd o)) /\ Rem? (snd (snd o3))) \/
-                    (Rem? (snd (snd o)) /\ Add? (snd (snd o3))) \/
-                    (Rem? (snd (snd o)) /\ Rem? (snd (snd o3)))) /\
-                    get_rid o <> get_rid o3)
-          (ensures eq (concrete_merge s s (do s' o)) (do s' o)) = ()*)
+////////////////////////////////////////////////////////////////
